Palphabeta.v
@@ -1,0 +1,387 @@
+From Stdlib Require Import ZArith Ascii List String PrimInt63.
+From Stdlib Require Import -(notations) PArray.
+From mathcomp Require Import all_boot.
+From HB Require Import structures.
+
+From Stdlib Require Import Lia.
+Require Import ssr_int.
+Require Import Pbasic.
+Require Import Pmoves.
+Require Import Phash.
+Require Import FourInARow.
+
+(******************************************************************************)
+(*                                                                            *)
+(*                                                                            *)
+(*    Alpha beta                                                              *)
+(*                                                                            *)
+(*                                                                            *)
+(******************************************************************************)
+
+
+Import PrimInt63Notations.
+Import Uint63Axioms.
+Import Uint63.
+Open Scope uint63_scope.
+
+(*
+(* Process result *)
+Inductive pres := PRes (s : int) (v : int) (t : array (array int)).
+*)
+
+
+Section Process.
+
+Variables w b : int.
+Variable beta : int.
+Variable lv  : int.
+Variable hg : int.
+Variable hs : int.
+Variable ab : int -> int -> int -> int -> int -> 
+                         array (array int) -> pres.
+Hypothesis hsV : valid_eval w b hs.
+Hypothesis hsL : hs land 1 == 0.
+Hypothesis wNw : ~~ cwin w.
+Hypothesis wNb : ~~ cwin b.
+Hypothesis wbWf : wf_state (w lor b).
+Hypothesis wbL : w land b = 0.
+
+Lemma ufixE v : ufix v land 1 = 1.
+Proof.
+rewrite /ufix; case: neqbP; first by apply: to_nat_inj.
+by case: neqbP.
+Qed.
+
+Lemma hs_range : [\/ hs = unknown, hs = lossdraw | hs = drawwin].
+Proof. by apply: valid_eval0E hsV _. Qed.
+
+Notation process := (process w b beta lv hg hs ab).
+
+Definition valid_ab a b :=
+  if a == loss then (b == draw) || (b == win) else (a == draw) && (b== win).
+
+Definition LOSSWIN := to_nat losswin.
+
+Lemma to_nat_rev_val a1 : 
+  a1 <=? losswin -> to_nat (rev_val a1) = (LOSSWIN - to_nat a1)%N.
+Proof. by move=> /nlebP a1Ll; rewrite to_nat_sub // to_nat_bounded. Qed.
+
+Lemma valid_ab_rev a1 b1 : valid_ab a1 b1 -> valid_ab (rev_val b1) (rev_val a1).
+Proof.
+rewrite /valid_ab; case: eqP => [-> /orP[]/eqP->//|_].
+by case: eqP => [-> /eqP->|].
+Qed.
+
+Definition valid_list (l : seq (int * int)) := forall m : int * int,
+    m \in l -> 
+    exists i j : nat, cmove (w lor b) i j /\
+    m.1 = lsl 1 (of_nat i * horizontal + of_nat j).
+
+Lemma valid_cons m (l : seq (int * int)) :
+   valid_list (m :: l) -> 
+    valid_list l /\ 
+    exists i j, cmove (w lor b) i j /\
+    m.1 = lsl 1 (of_nat i * horizontal + of_nat j).
+Proof.
+by move=> lV; split => [m1 m1Il|]; apply: lV; rewrite inE ?eqxx ?m1Il ?orbT.
+Qed.
+
+Hypothesis ab_correct : forall w b alpha1 beta1 sc v v1 h h1, 
+  valid_hash_table h ->
+  valid_ab alpha1 beta1 ->
+  ab w b alpha1 beta1 v h =  PRes sc v1 h1 ->
+  [/\ sc != unknown, valid_hash_table h1 & valid_eval w b sc].
+
+Lemma cmove_has_move wb i j : cmove wb i j -> has_move wb.
+Proof.
+move=> ijM.
+have iLw : i < nwidth by case/and3P: ijM.
+have jLh : j < nheight by case/and3P: ijM.
+by apply/existsP; exists (Ordinal iLw); apply/existsP; exists (Ordinal jLh).
+Qed.
+
+Lemma leq_eval_move i j : 
+  cmove (w lor b) i j -> wcomp (eval b (mk_move w i j)) <= eval w b.
+Proof.
+move => ijM.
+have iLw : i < nwidth by case/and3P: ijM.
+have jLh : j < nheight by case/and3P: ijM.
+rewrite [X in _ <= X]evalS /= (negPf wNw) ifT; last by apply: cmove_has_move ijM.
+rewrite (bigD1 (Ordinal iLw)) //= (leq_trans  _ (leq_maxl _ _)) //.
+by rewrite (bigD1 (Ordinal jLh)) //= leq_maxl.
+Qed.
+
+Lemma leq_wcomp a1 b1 : a1 <= b1 -> wcomp b1 <= wcomp a1.
+Proof. by move=> a1Lb1; rewrite leq_sub. Qed.
+
+Lemma leq_eval_win w1 b1 : eval w1 b1 <= WIN.
+Proof. by have /or3P[] := evalOr w1 b1 => /eqP->. Qed.
+
+Lemma leq_loss_eval w1 b1 : LOSS <= eval w1 b1.
+Proof. by have /or3P[] := evalOr w1 b1 => /eqP->. Qed.
+
+Lemma process_correct  ms alpha sc sc1 v v1 h h1:
+  valid_list ms -> valid_hash_table h -> valid_ab alpha beta ->
+  process ms alpha sc v h =  PRes sc1 v1 h1 ->
+  valid_hash_table h1.
+Proof.
+elim: ms alpha sc sc1 v v1 h h1 =>
+   [|[m x] ms IH] alpha sc sc1 v v1 h h1 Vms Vh Vab /=.
+  case: neqbP.
+    move=> HH.
+    suff eD : DRAW <= eval w b <= DRAW.
+      by case => dE _ <-; apply: valid_has_table_valid_hput.
+    admit.
+  move=> HH.
+  suff eD : down_score sc <= eval w b <= up_score sc.
+    case => dE _ <-.
+    by apply: valid_has_table_valid_hput.
+  admit.
+case E : ab => [s2 v2 h2].
+case: (ab_correct _ _ _ _ _ _ _ _ _ _ _ E) => // [|s2Nu h2V vEs2].
+  by apply: valid_ab_rev.
+have [Vms1 [i [j [ijM mE]]]] := valid_cons _ _ Vms. 
+have mmE : make_move m w = mk_move w i j.
+  by rewrite [m]mE /mk_move /make_move lorC.
+have us2Le : wcomp (up_score s2) <= eval w b.
+  have /(leq_trans _)-> // := leq_eval_move _ _ ijM.
+  by apply: leq_wcomp; rewrite -mmE; case/andP: vEs2.
+case: nltbP => [rs2Lb|/negP].
+  case: nlebP => _; first by apply: IH.
+  case: nlebP => [_|/negP]; first by apply: IH.
+  rewrite -ltnNge => aLrs2. 
+  apply: IH => //.
+  have betaE : (beta == draw) || (beta == win).
+    by move: Vab; rewrite /valid_ab; case: eqP => // _ /andP[_ ->]; rewrite orbT.
+  have alphaE : (alpha == loss) || (alpha == draw).
+    by move: Vab; rewrite /valid_ab; case: eqP => // _ /andP[].
+  rewrite /valid_ab.
+  have := rs2Lb.
+  by have [] := valid_evalE _ _ _ vEs2; case=> -> //=;
+    case/orP : betaE => /eqP-> //.
+rewrite -leqNgt => bLrs2.
+case: nlebP => _; first by apply: IH.
+case: nlebP => [_|/negP]; first by apply: IH.
+rewrite -ltnNge => aLrs2.
+case: (neqbP _ draw) => rs2Ed; last first.
+  rewrite andFb.
+  case: neqbP => rs2El.
+    have s2E : s2 = lossdraw.
+      by have := rs2El; have [] := valid_evalE _ _ _ vEs2 => [] [] ->.
+    case: neqbP => hsE.
+      suff eD : DRAW <= eval w b <= DRAW.
+        rewrite andTb; case => dE _ <-.
+        by apply: valid_has_table_valid_hput => //.
+      have hsE1 : hs = lossdraw by apply: to_nat_inj.
+      have {vEs2} := vEs2.
+      rewrite s2E /valid_eval -[down_score _]/LOSS -[up_score _]/DRAW => vEs2.
+      have := hsV.
+      rewrite hsE1 /valid_eval -[down_score _]/LOSS -[up_score _]/DRAW => hsV1.
+      apply/andP; split; last by case/andP: hsV1.
+      by have := us2Le; rewrite s2E. 
+    suff eD : down_score (rev_val s2) <= eval w b <= up_score (rev_val s2).
+      rewrite andTb; case => dE _ <-.
+      by apply: valid_has_table_valid_hput.
+    have {vEs2} := vEs2.
+    rewrite s2E /valid_eval -[down_score _]/LOSS -[up_score _]/DRAW => vEs2.
+    rewrite -[down_score _]/DRAW -[up_score _]/WIN.
+    apply/andP; split; last by apply: leq_eval_win.
+    by have := us2Le; rewrite s2E.  
+  suff eD : down_score (rev_val s2) <= eval w b <= up_score (rev_val s2).
+    rewrite andFb; case => dE _ <-.
+    by apply: valid_has_table_valid_hput.
+  have s2El : s2 = loss.
+    move: bLrs2 rs2Ed rs2El.
+    have /orP[/eqP->|/eqP->] : (beta == draw) || (beta == win).
+    - by move: Vab; rewrite /valid_ab; case: eqP => // _ /andP[_ ->]; rewrite orbT.
+    - by move/valid_evalE: vEs2; case; case => ->.
+    by move/valid_evalE: vEs2; case; case => ->.
+  suff -> : eval w b = WIN by rewrite s2El.
+  apply/eqP/eval_winP; right.
+  exists i; exists j; split => //.
+  rewrite -mmE.
+  move: vEs2; rewrite /valid_eval s2El.
+  by have /or3P[] := evalOr b (make_move m w) => /eqP->.
+have s2E : s2 = draw.
+  by move: rs2Ed; move/valid_evalE: vEs2; case; case => ->.
+case: (boolP (is_nempty_move ms)) => ems.
+  rewrite andTb eqb_refl.
+  case: neqbP => hD.
+    have hsE : hs = lossdraw by apply: to_nat_inj.
+    suff eD : DRAW <= eval w b <= DRAW.
+      by case => dE _ <-; apply: valid_has_table_valid_hput.
+    apply/andP; split; last first.
+      by move: hsV; rewrite /valid_eval hsE; case/andP.
+    by have := us2Le; rewrite s2E.
+  suff eD : DRAW <= eval w b <= WIN.
+    by case => dE _ <-; apply: valid_has_table_valid_hput.
+  apply/andP; split; last by apply: leq_eval_win.
+  by have := us2Le; rewrite s2E.
+suff eD : DRAW <= eval w b <= DRAW.
+  rewrite s2E andFb; case => dE _ <-.
+  by apply: valid_has_table_valid_hput.
+admit.
+Qed.
+
+Variables (wstate bstate : int) (beta : int) (lvisited : int) 
+          (height hscore :  int)
+          (alpha_beta : int -> int -> int -> int -> int -> 
+                         array (array int) -> pres).
+Fixpoint process ms alpha score visited hash_table :=
+  match ms with
+  | EmptyMove =>
+      let score := if (score =? losswin - hscore) then draw else score in
+      let work := log2 (sub visited lvisited) in
+      let hash_table := hput wstate bstate turn work score hash_table height in
+      PRes score (incr visited) hash_table
+  | Move move _ ms1 =>
+    let (nscore,visited,hash_table) := 
+      alpha_beta bstate (make_move move wstate) (negb turn)
+           (rev_val beta) (rev_val alpha) visited hash_table in
+    let nscore := rev_val nscore in
+    if nscore <=? score then process ms1 alpha score visited hash_table 
+    else
+    let score := nscore in
+    if score <=? alpha then process ms1 alpha score visited hash_table                 
+    else
+    let alpha := score in
+    if alpha <? beta  then process ms1 alpha score visited hash_table 
+    else
+      let score :=
+        if (andb (score =? draw) (is_nempty_move ms1)) then drawwin 
+        else score in
+      let score := if (score =? losswin - hscore) then draw else score in
+      let work := log2 (sub visited  lvisited) in
+      let hash_table := hput wstate bstate turn work score hash_table height in
+      PRes score (incr visited) hash_table
+    end.
+
+End Process.
+
+(* alpha-beta result *)
+Inductive ares := ARes (a : int) (b : int) (c : bool).
+
+Section Alpha.
+
+(* alpha beta pruning search *)
+Fixpoint alpha_beta nstruct height wstate bstate turn alpha beta 
+                    visited hash_table :=
+  let hscore := hget wstate bstate turn hash_table height in
+  let (alpha,beta,flag) :=
+    (if (hscore =? unknown) then ARes alpha beta false else
+    if negb ((hscore land 1) =? 0) then ARes alpha beta true else
+    if (hscore =? drawwin) then
+      if (beta =? draw) then ARes alpha beta true else ARes draw beta false
+    else
+      if (alpha =? draw) then ARes alpha beta true 
+      else ARes alpha draw false) in
+  if flag then PRes hscore visited hash_table else
+  match find_moves wstate bstate with
+  | Win => PRes win visited hash_table
+  | Draw => PRes draw visited hash_table
+  | Forced move =>
+      match nstruct with 
+     | 0%nat => PRes unknown visited hash_table
+     | S nstruct =>
+      let (score,visited,hash_table) := 
+        alpha_beta nstruct (height + 1) bstate (make_move move wstate) 
+                   (negb turn) (rev_val beta) (rev_val alpha) 
+                    visited hash_table : pres in
+      PRes (rev_val score) visited hash_table 
+     end
+  | Moves ms =>
+     match nstruct with 
+     | 0%nat => PRes unknown visited hash_table
+     | S nstruct =>
+     process wstate bstate turn beta visited height hscore 
+            (alpha_beta nstruct (height + 1))
+             ms alpha loss visited hash_table
+     end
+  end.
+
+Lemma alpha_betaE nstruct height wstate bstate turn alpha beta 
+                    visited hash_table  :
+ alpha_beta nstruct height wstate bstate turn alpha beta 
+                    visited hash_table =
+  let hscore := hget wstate bstate turn hash_table height in
+  let (alpha,beta,flag) :=
+    (if (hscore =? unknown) then ARes alpha beta false else
+    if negb ((hscore land 1) =? 0) then ARes alpha beta true else
+    if (hscore =? drawwin) then
+      if (beta =? draw) then ARes alpha beta true else ARes draw beta false
+    else
+      if (alpha =? draw) then ARes alpha beta true 
+      else ARes alpha draw false) in
+  if flag then PRes hscore visited hash_table else
+  match find_moves wstate bstate with
+  | Win => PRes win visited hash_table
+  | Draw => PRes draw visited hash_table
+  | Forced move =>
+      match nstruct with 
+     | 0%nat => PRes unknown visited hash_table
+     | S nstruct =>
+      let (score,visited,hash_table) := 
+        alpha_beta nstruct (height + 1) bstate (make_move move wstate) 
+                   (negb turn) (rev_val beta) (rev_val alpha) 
+                    visited hash_table : pres in
+      PRes (rev_val score) visited hash_table 
+     end
+  | Moves ms =>
+     match nstruct with 
+     | 0%nat => PRes unknown visited hash_table
+     | S nstruct =>
+     process wstate bstate turn beta visited height hscore 
+            (alpha_beta nstruct (height + 1))
+             ms alpha loss visited hash_table
+     end
+  end.
+Proof. by case: nstruct. Qed.
+
+Definition eval_position s :=
+   match parse_string s with
+   (wstate,bstate,turn) =>
+   let (wstate,bstate) := if turn then (wstate,bstate) else (bstate,wstate) in
+   let (score, _, _) :=
+     alpha_beta (1 + nheight * nwidth)%nat 0 wstate bstate turn loss win zero
+                (make_hash tt) in
+   score
+   end.
+
+End Alpha.
+
+Definition ex1 := (
+                 "___O___"
+              ++ "___X___"
+              ++ "___O___"
+              ++ "___X___"
+              ++ "__OO___"
+              ++ "__XX___")%string.
+
+
+Definition ex2 := (
+                 "___X___"
+              ++ "__OX___"
+              ++ "__XO___"
+              ++ "__OX___"
+              ++ "__XO___"
+              ++ "__OX__O")%string.
+
+
+Definition ex3 := (
+                 "___O___"
+              ++ "___X___" 
+              ++ "___O___"
+              ++ "___X___"
+              ++ "___O___"
+              ++ "XO_X___")%string.
+
+Definition ex4 := ("______" ++ "______" ++ "______" ++
+                   "______" ++ "______" ++ "______" ++ "______")%string.
+
+(*
+Time Eval native_compute in string_of_score (eval_position ex1).
+Time Eval native_compute in string_of_score (eval_position ex2).
+Time Eval native_compute in string_of_score (eval_position ex3).
+Time Eval native_compute in string_of_score (eval_position ex4).
+
+*)
